src/Noninterference/SelfSimulationExists.v
@@ -1,0 +1,205 @@
+Require Import Framework File FileDiskLayer FileDiskNoninterference FileDiskRefinement.
+Require Import FunctionalExtensionality Lia.
+
+Definition AD_valid_state := refines_to_valid FileDiskRefinement FD_valid_state.
+Definition AD_related_states u exc := refines_to_related FileDiskRefinement (FD_related_states u exc).
+
+Ltac econstructor_recovery :=
+  match goal with
+  | [|- recovery_exec _ ?u [?o] _ [] _ _ _ ]=>
+    eapply (@ExecFinished _ _ _ _ u o)
+  | [|- recovery_exec _ ?u (?o :: _) _ (?rf :: _) _ _ _ ]=>
+    eapply (@ExecRecovered _ _ _ _ u o _ _ _ rf)
+  end.
+
+Theorem SelfSimulation_Exists_recover:
+  forall u n,
+      SelfSimulation_Exists u recover recover recover
+                            AD_valid_state (AD_related_states u None)
+                            (authenticated_disk_reboot_list n).
+Proof.
+  induction n; simpl;
+  unfold SelfSimulation_Exists, AD_valid_state,
+  AD_related_states, FD_valid_state, FD_related_states,
+  refines_to_valid, refines_to_related,
+  authenticated_disk_reboot_list in *;
+  intros; cleanup; simpl in *.
+  {
+    invert_exec; cleanup.
+    unfold recover in *; repeat invert_exec; simpl in *.
+    invert_exec'' H11; simpl in *.
+    repeat invert_exec.
+    eexists.    
+    econstructor_recovery.
+    repeat econstructor.
+  }
+  {
+    invert_exec; cleanup.
+    unfold recover in *; repeat invert_exec; simpl in *.
+    invert_exec'' H14; simpl in *.
+    repeat invert_exec.
+    repeat cleanup_pairs.    
+    destruct s2, s1; simpl in *.
+    edestruct IHn.
+    3: apply H15.
+    intros; eauto.
+    intros; eauto.    
+    instantiate (1:= (s0, (t2, t2))).
+    unfold refines_to, files_rep in *; simpl in *.
+    cleanup; do 2 eexists; intuition eauto.
+    eexists.
+    econstructor_recovery.
+    repeat econstructor; eauto.
+    simpl; eauto.
+  }
+Qed.
+
+Theorem SelfSimulation_Exists_auth_then_exec:
+  forall u m inum T (p1 p2: Inode.Inum -> prog (TransactionalDiskLayer.TransactionalDiskLang FSParameters.data_length) (option T)) ex,
+    (forall n, SelfSimulation_Exists u (lift_L2 _ (p1 inum)) (lift_L2 _ (p2 inum)) recover
+        AD_valid_state (AD_related_states u ex)
+        (authenticated_disk_reboot_list n)) ->
+    
+    SelfSimulation_Exists
+      u (auth_then_exec inum p1) (auth_then_exec inum p2) recover
+      AD_valid_state (AD_related_states u ex)
+      (authenticated_disk_reboot_list m).
+Proof.
+  unfold SelfSimulation_Exists, AD_valid_state,
+  AD_related_states, FD_valid_state, FD_related_states,
+  refines_to_valid, refines_to_related,
+  authenticated_disk_reboot_list;
+  intros; cleanup; simpl in *.
+  destruct m; simpl in *.
+  {
+    unfold auth_then_exec in *; repeat invert_exec; cleanup.
+    invert_exec'' H12; simpl in *; cleanup; repeat invert_exec.
+    {
+      invert_exec'' H11; simpl in *; cleanup; repeat invert_exec.
+      {
+        invert_exec'' H16; simpl in *; cleanup; repeat invert_exec.
+        invert_exec'' H12; simpl in *; cleanup; repeat invert_exec.
+        {
+          invert_exec'' H16; simpl in *; cleanup; repeat invert_exec.
+          unfold Inode.InodeAllocator.read in *; cleanup; repeat invert_exec.
+          {
+            invert_exec'' H11; simpl in *; cleanup; repeat invert_exec.
+            { 
+              invert_exec'' H12; simpl in *; cleanup; repeat invert_exec.
+              {
+                invert_exec'' H16; simpl in *; cleanup; repeat invert_exec.
+                invert_exec'' H17; simpl in *; cleanup; repeat invert_exec.
+                invert_exec'' H12; simpl in *; cleanup; repeat invert_exec.
+                {
+                  cleanup.
+                  invert_exec'' H15; simpl in *; cleanup; repeat invert_exec.
+                  {
+                    invert_exec'' H12; simpl in *; cleanup; repeat invert_exec.
+                    {
+                      invert_exec'' H17; simpl in *; cleanup; repeat invert_exec.
+                      {
+                        invert_exec'' H16; simpl in *; cleanup; repeat invert_exec.
+                        invert_exec'' H18; simpl in *; cleanup; repeat invert_exec.
+                        invert_exec'' H14; simpl in *; cleanup; repeat invert_exec.
+                        edestruct (H 0); simpl in *.
+                        3: {
+                          eapply (@ExecFinished _ _ _ _
+                                 (Inode.owner (Inode.decode_inode (fst (snd s1)
+                                 (Inode.InodeAllocatorParams.bitmap_addr + S inum)))) o1 _ _); eauto.
+                        }
+                        all: intros; eauto.
+                        eexists; simpl.
+                        econstructor_recovery.
+                        simpl.
+                        replace (OpToken
+       (HorizontalComposition AuthenticationLayer.AuthenticationOperation
+          (TransactionalDiskLayer.TransactionalDiskOperation FSParameters.data_length))
+       (Token2 AuthenticationLayer.AuthenticationOperation
+          (TransactionalDiskLayer.TransactionalDiskOperation FSParameters.data_length)
+          TransactionalDiskLayer.Cont)
+     :: OpToken
+          (HorizontalComposition AuthenticationLayer.AuthenticationOperation
+             (TransactionalDiskLayer.TransactionalDiskOperation FSParameters.data_length))
+          (Token2 AuthenticationLayer.AuthenticationOperation
+             (TransactionalDiskLayer.TransactionalDiskOperation FSParameters.data_length)
+             TransactionalDiskLayer.Cont)
+        :: Language.Cont
+             (HorizontalComposition AuthenticationLayer.AuthenticationOperation
+                (TransactionalDiskLayer.TransactionalDiskOperation FSParameters.data_length))
+           :: Language.Cont
+                (HorizontalComposition AuthenticationLayer.AuthenticationOperation
+                   (TransactionalDiskLayer.TransactionalDiskOperation FSParameters.data_length))
+              :: Language.Cont
+                   (HorizontalComposition AuthenticationLayer.AuthenticationOperation
+                      (TransactionalDiskLayer.TransactionalDiskOperation FSParameters.data_length))
+                 :: OpToken
+                      (HorizontalComposition AuthenticationLayer.AuthenticationOperation
+                         (TransactionalDiskLayer.TransactionalDiskOperation FSParameters.data_length))
+                      (Token1 AuthenticationLayer.AuthenticationOperation
+                         (TransactionalDiskLayer.TransactionalDiskOperation FSParameters.data_length)
+                         AuthenticationLayer.Cont)
+                    :: o1 ++
+                       [OpToken
+                          (HorizontalComposition AuthenticationLayer.AuthenticationOperation
+                             (TransactionalDiskLayer.TransactionalDiskOperation FSParameters.data_length))
+                          (Token2 AuthenticationLayer.AuthenticationOperation
+                             (TransactionalDiskLayer.TransactionalDiskOperation FSParameters.data_length)
+                             TransactionalDiskLayer.Cont);
+                       Language.Cont
+                         (HorizontalComposition AuthenticationLayer.AuthenticationOperation
+                                                (TransactionalDiskLayer.TransactionalDiskOperation FSParameters.data_length))])
+                          with
+   (((([OpToken (HorizontalComposition AuthenticationLayer.AuthenticationOperation
+          (TransactionalDiskLayer.TransactionalDiskOperation FSParameters.data_length))
+       (Token2 AuthenticationLayer.AuthenticationOperation
+          (TransactionalDiskLayer.TransactionalDiskOperation FSParameters.data_length)
+          TransactionalDiskLayer.Cont)] ++
+    ([OpToken
+      (HorizontalComposition AuthenticationLayer.AuthenticationOperation
+         (TransactionalDiskLayer.TransactionalDiskOperation FSParameters.data_length))
+      (Token2 AuthenticationLayer.AuthenticationOperation
+         (TransactionalDiskLayer.TransactionalDiskOperation FSParameters.data_length)
+         TransactionalDiskLayer.Cont)] ++
+    [Language.Cont
+      (HorizontalComposition AuthenticationLayer.AuthenticationOperation
+         (TransactionalDiskLayer.TransactionalDiskOperation FSParameters.data_length))])) ++
+    [Language.Cont
+      (HorizontalComposition AuthenticationLayer.AuthenticationOperation
+         (TransactionalDiskLayer.TransactionalDiskOperation FSParameters.data_length))]) ++
+    [Language.Cont
+      (HorizontalComposition AuthenticationLayer.AuthenticationOperation
+         (TransactionalDiskLayer.TransactionalDiskOperation FSParameters.data_length))]) ++
+    (OpToken (HorizontalComposition AuthenticationLayer.AuthenticationOperation
+            (TransactionalDiskLayer.TransactionalDiskOperation FSParameters.data_length))
+            (Token1 AuthenticationLayer.AuthenticationOperation
+             (TransactionalDiskLayer.TransactionalDiskOperation FSParameters.data_length)
+              AuthenticationLayer.Cont) :: o1 ++
+    [OpToken
+       (HorizontalComposition AuthenticationLayer.AuthenticationOperation
+        (TransactionalDiskLayer.TransactionalDiskOperation FSParameters.data_length))
+       (Token2 AuthenticationLayer.AuthenticationOperation
+        (TransactionalDiskLayer.TransactionalDiskOperation FSParameters.data_length)
+        TransactionalDiskLayer.Cont);
+     Language.Cont
+       (HorizontalComposition AuthenticationLayer.AuthenticationOperation
+       (TransactionalDiskLayer.TransactionalDiskOperation FSParameters.data_length))])).
+
+   repeat eapply ExecBind.
+   repeat econstructor; eauto.
+   {
+     clear H H0 H1.
+     unfold refines_to, files_rep,
+     files_inner_rep, file_map_rep,
+     Inode.inode_rep,
+     Inode.InodeAllocator.block_allocator_rep,
+     Inode.inode_map_rep in *;
+     cleanup.
+     eapply Inode.InodeAllocator.valid_bits_extract with (n := inum) in v0; eauto;
+     try lia.          
+     cleanup.
+     eapply nth_error_nth with (d:= false) in D0; eauto.
+     rewrite <- nth_selN_eq in D0.
+     setoid_rewrite equal_f with (x5 :=  Inode.InodeAllocatorParams.bitmap_addr) in D0; eauto.
+     split_ors; cleanup; try congruence.
+     setoid_rewrite H0 in D0; congruence.
+     
