src/Refinements/LogCacheToLoggedDisk/Simulations.v
@@ -1,0 +1,486 @@
+Require Import Framework TotalMem FSParameters CachedDiskLayer.
+Require Import Log RepImplications Specs LogCache LoggedDiskLayer.
+Require Import LogCacheToLoggedDisk.Definitions LogCacheToLoggedDisk.AbstractOracles.
+Require Import ClassicalFacts FunctionalExtensionality Lia.
+
+Set Nested Proofs Allowed.
+
+Local Notation "'imp'" := CachedDiskLang.
+Local Notation "'abs'" := (LoggedDiskLang log_length data_length).
+Local Notation "'refinement'" := LoggedDiskRefinement.
+
+  Lemma ext_or_take_out:
+    forall A P Q R,
+      (exists a: A, P a) \/ (exists a: A, Q a) \/ (exists a : A, R a)->
+      exists a: A, P a \/ Q a \/ R a.
+  Proof.
+    intros; intuition (cleanup; eauto).
+  Qed.
+
+  
+  
+Lemma recovery_simulation :
+  forall l_selector u,
+    SimulationForProgramGeneral _ _ _ _ refinement u _ (|Recover|) (|Recover|)
+                         (cached_disk_reboot_list l_selector)
+                         (logged_disk_reboot_list (length l_selector))
+                         refines_to_reboot refines_to.
+Proof.
+  unfold SimulationForProgramGeneral; induction l_selector; simpl; intros; cleanup.
+  {
+    destruct l_o_imp; intuition; simpl in *.
+    cleanup; intuition.
+    invert_exec; simpl in *; cleanup; intuition.
+    specialize H2 with (1:= H12).
+    cleanup; intuition eauto; cleanup; try unify_execs; cleanup.
+    
+    eexists; intuition eauto.
+    unfold logged_disk_reboot_list in *; simpl.
+    simpl in *; destruct l; simpl in *; try lia.
+    instantiate (1:= RFinished s_abs tt). 
+    repeat econstructor.
+    unfold refines_to, refines_to_reboot in *;
+    simpl in *; cleanup; eauto.
+    simpl; eauto.
+  }
+  {
+    invert_exec; simpl in *; cleanup; intuition;
+    cleanup; intuition eauto; repeat (unify_execs; cleanup).
+    clear H1.
+    specialize H2 with (1:= H11).
+    cleanup; intuition eauto; cleanup; try unify_execs; cleanup.
+    edestruct IHl_selector; eauto.
+    instantiate (1:= s_abs).
+    all: eauto.
+    unfold refines_to_reboot in *; logic_clean.
+    eapply_fresh recover_crashed in H11; eauto.
+    cleanup; simpl in *; split; eauto.
+    unfold cached_log_reboot_rep in *; cleanup.
+
+    eapply ext_or_take_out in H3.
+    cleanup.
+    exists x1.
+    simpl; split.
+    cleanup; repeat split_ors;
+    simpl in *; cleanup;
+    try eapply reboot_rep_to_reboot_rep in H3;
+    try eapply crash_rep_recover_to_reboot_rep in H3;
+    try eapply log_rep_to_reboot_rep in H3;
+    intuition eauto.
+     
+    assert (A: (map addr_list x1) = (map (map (Nat.add data_start)) (map (map (fun a => a - data_start)) (map addr_list x1)))). {
+        rewrite map_map.
+        setoid_rewrite map_ext_in at 2.
+        rewrite map_id; eauto.
+        intros.
+        rewrite map_map.
+        setoid_rewrite map_ext_in.
+        rewrite map_id; eauto.
+        intros; simpl.
+        unfold log_rep, log_rep_general, log_crash_rep,
+        log_reboot_rep, log_rep_explicit,
+        log_rep_inner, txns_valid in *.
+        simpl in *; logic_clean.
+        repeat split_ors; cleanup;
+        match goal with
+        | [H: Forall (txn_well_formed _ _ _ _ _) _,
+              H0: In _ (map _ _) |- _] =>
+          apply in_map_iff in H0; logic_clean; subst;
+          eapply Forall_forall in H; eauto;
+          unfold txn_well_formed in H; logic_clean
+        end;
+        match goal with
+        |[H: Forall (fun _ => _ > _ /\ _ >= _) _ |- _] =>
+         eapply Forall_forall in H; eauto
+        end;
+        lia.
+      }
+      simpl.
+      rewrite A.
+      rewrite shift_list_upd_batch_set_comm.
+      rewrite <- shift_select_total_mem_comm.
+      rewrite select_total_mem_synced_noop.
+      rewrite <- shift_list_upd_batch_set_comm.
+      setoid_rewrite <- A; eauto.
+      repeat split_ors; logic_clean; eauto;
+      
+      repeat rewrite total_mem_map_shift_comm in *;
+      rewrite <- sync_list_upd_batch_set in H6;
+      rewrite total_mem_map_fst_sync_noop in H6;
+      eauto.
+      
+      {
+        unfold sumbool_agree; intros.
+        destruct (addr_dec x2 y); subst.
+        destruct (addr_dec (data_start + y) (data_start + y)); eauto; congruence.
+        destruct (addr_dec (data_start + x2) (data_start + y)); eauto; lia.
+      }
+      {
+        intros.
+        rewrite shift_some in H6.
+        split_ors;
+        rewrite H5 in H6; eauto.
+        lia.
+        unfold sync in H6.
+        destruct_fresh (snd (snd s_imp) (data_start + a0));
+        setoid_rewrite D in H6; inversion H6; simpl; eauto.
+        lia.
+      }
+      {
+        unfold sumbool_agree; intros.
+        destruct (addr_dec x2 y); subst.
+        destruct (addr_dec (data_start + y) (data_start + y)); eauto; congruence.
+        destruct (addr_dec (data_start + x2) (data_start + y)); eauto; lia.
+      }
+      simpl in *.
+      intros.
+      eapply select_total_mem_synced in H6; eauto.
+      
+      simpl in *; logic_clean.
+      exists (Recovered (extract_state_r x)).
+      unfold logged_disk_reboot_list in *; simpl in *.
+      econstructor.
+      repeat econstructor; eauto.
+      eauto.
+  }
+Qed. 
+
+Lemma read_simulation :
+  forall a l_selector u,
+    SimulationForProgram refinement u (|Read a|) (|Recover|)
+                         (cached_disk_reboot_list l_selector)
+                         (logged_disk_reboot_list (length l_selector)).
+Proof.
+  unfold SimulationForProgram, SimulationForProgramGeneral; simpl; intros; cleanup.
+  
+    invert_exec; simpl in *; cleanup; intuition;
+    cleanup; try solve [intuition eauto; try congruence;
+                        unify_execs; cleanup].
+    {
+      specialize H1 with (1:= H10).
+      cleanup; intuition eauto; cleanup; try unify_execs; cleanup.
+      eapply_fresh read_finished in H10; cleanup; eauto.
+      destruct l_selector; simpl in *; try congruence; cleanup.
+      destruct l; simpl in *; try lia.
+      unfold logged_disk_reboot_list; simpl.
+      split_ors; cleanup.
+      {
+        exists (RFinished s_abs (s_abs a));
+        simpl; intuition eauto.
+        eapply ExecFinished.
+        repeat econstructor; eauto.
+      }
+      {
+        exists (RFinished s_abs value0);
+        simpl; intuition eauto.
+        eapply ExecFinished.
+        repeat econstructor; eauto.
+      }
+    }
+    {
+      clear H1.
+      specialize H3 with (1:= H9).
+      cleanup; intuition eauto; cleanup; try unify_execs; cleanup.
+      destruct l_selector; simpl in *; try congruence; cleanup.
+      eapply_fresh read_crashed in H9; cleanup.
+      
+      edestruct recovery_simulation; eauto.
+      unfold refines_to in *.
+      apply H4 in H0.
+      unfold refines_to_reboot; simpl.
+      instantiate (1:= s_abs).
+      unfold cached_log_rep, cached_log_reboot_rep in *; cleanup.
+      eapply_fresh log_rep_to_reboot_rep in H1.
+      intuition eauto.
+      eexists; intuition eauto.
+      simpl; eauto.
+
+      unfold log_rep, log_reboot_rep, log_rep_general in *.
+      logic_clean.
+      setoid_rewrite map_addr_list_eq_map_map at 2; eauto.
+      rewrite shift_list_upd_batch_set_comm; eauto.
+      rewrite shift_select_total_mem_synced.      
+      repeat rewrite <- shift_list_upd_batch_set_comm.        
+      repeat erewrite <- map_addr_list_eq_map_map; eauto.
+      
+      all: try apply sumbool_agree_addr_dec.
+      intros; apply H5; lia.
+      apply select_total_mem_synced in H3; eauto.
+      
+      exists (Recovered (extract_state_r x)); simpl; intuition eauto.
+      unfold logged_disk_reboot_list; simpl.
+      eapply ExecRecovered; eauto.
+      repeat econstructor.
+    }
+Qed.
+
+Lemma write_simulation :
+  forall l_a l_v l_selector u,
+    SimulationForProgram refinement u (|Write l_a l_v|) (|Recover|)
+                         (cached_disk_reboot_list l_selector)
+                         (logged_disk_reboot_list (length l_selector)).
+Proof.
+  unfold SimulationForProgram, SimulationForProgramGeneral; simpl; intros; cleanup.
+  
+    invert_exec; simpl in *; cleanup; intuition;
+    cleanup; try solve [intuition eauto; try congruence;    
+    unify_execs; cleanup].
+    {
+      specialize H1 with (1:= H10).
+      cleanup; intuition eauto; cleanup; try unify_execs; cleanup.
+      {
+        eapply write_finished in H10; eauto.
+        destruct l_selector; simpl in *; try congruence; cleanup.
+        destruct l; simpl in *; try lia.
+        unfold logged_disk_reboot_list; simpl.
+        split_ors; cleanup.
+        {
+          exists (RFinished s_abs tt);
+          simpl; split; eauto.
+          eapply ExecFinished.
+          do 2 econstructor; eauto.
+          intuition eauto.
+          erewrite addr_list_to_blocks_length_eq; eauto.
+          rewrite map_length; eauto.
+          destruct x1; eauto.
+        }
+      {
+        exists (RFinished (upd_batch s_abs l_a l_v) tt);
+        simpl; intuition eauto.
+        eapply ExecFinished.
+        repeat econstructor; eauto.
+        erewrite addr_list_to_blocks_length_eq; eauto.
+        rewrite map_length; eauto.
+        destruct x1; eauto.
+      }
+    }
+    {
+      split_ors; cleanup;
+      try unify_execs; cleanup;
+      destruct l_selector; simpl in *; try congruence; cleanup.
+      split_ors; cleanup;
+      try unify_execs; cleanup;
+      destruct l_selector; simpl in *; try congruence; cleanup.
+    }
+    }
+    {
+      unfold refines_to in *.
+      clear H1.
+      specialize H3 with (1:= H9).
+      cleanup; intuition eauto; cleanup; try unify_execs; cleanup.
+      destruct l_selector; simpl in *; try congruence; cleanup.
+      
+      repeat split_ors; cleanup; try unify_execs; cleanup.
+      {
+        specialize H4 with (1:= H0).
+        repeat split_ors.
+        {
+          unfold cached_log_rep in *; cleanup.
+          edestruct recovery_simulation; eauto;
+          try solve [eapply H3; eauto].
+          {
+            unfold refines_to_reboot, cached_log_reboot_rep; simpl.
+            split.          
+            eapply log_rep_to_reboot_rep in H3.
+            eexists; intuition eauto.
+            intros.
+            apply select_total_mem_synced in H7; eauto.
+          }
+          {
+          exists (Recovered (extract_state_r x2)); simpl; intuition eauto.        
+          unfold logged_disk_reboot_list; simpl.
+          eapply ExecRecovered.
+          repeat econstructor.
+          unfold refines_to, cached_log_rep in *; cleanup.
+          unfold log_rep, log_reboot_rep, log_rep_general in *.
+          logic_clean.
+          erewrite map_addr_list_eq_map_map; eauto.
+          rewrite shift_list_upd_batch_set_comm; eauto.
+          erewrite <- shift_select_total_mem_synced.      
+          repeat rewrite <- shift_list_upd_batch_set_comm.        
+          repeat erewrite <- map_addr_list_eq_map_map; eauto.
+          
+          all: try apply sumbool_agree_addr_dec.
+          intros; apply H5; lia.
+          }
+      }
+        { (** During Apply Case **)
+          unfold cached_log_crash_rep in *; cleanup.
+          eapply crash_rep_apply_to_reboot_rep in H1.
+          repeat split_ors; edestruct recovery_simulation; eauto;
+          try solve [eapply H3; eauto].
+          {
+            unfold refines_to_reboot, cached_log_reboot_rep; simpl.          
+            split.          
+            eexists; intuition eauto.
+            intros.
+            apply select_total_mem_synced in H3; eauto.
+          }
+          {
+            
+            exists (Recovered (extract_state_r x1)); simpl; intuition eauto.        
+            unfold logged_disk_reboot_list; simpl.
+            eapply ExecRecovered.
+            repeat econstructor.
+            unfold refines_to, cached_log_rep in *; cleanup.
+            unfold log_rep, log_reboot_rep, log_rep_general in *.
+            logic_clean.
+            erewrite map_addr_list_eq_map_map; eauto.
+            rewrite shift_list_upd_batch_set_comm; eauto.
+            erewrite <- shift_select_total_mem_synced.      
+            repeat rewrite <- shift_list_upd_batch_set_comm.        
+            repeat erewrite <- map_addr_list_eq_map_map; eauto.
+            
+            all: try apply sumbool_agree_addr_dec.
+            (** Investigate this further **)
+            admit.
+          }
+          {
+            unfold refines_to_reboot, cached_log_reboot_rep; simpl.          
+            split.
+            eexists; intuition eauto.
+            intros.
+            apply select_total_mem_synced in H3; eauto.
+          }
+          {
+            exists (Recovered (extract_state_r x1)); simpl; intuition eauto.        
+            unfold logged_disk_reboot_list; simpl.
+            eapply ExecRecovered.
+            repeat econstructor.
+            unfold refines_to, cached_log_rep in *; cleanup.
+            simpl in *.
+            unfold log_rep, log_reboot_rep, log_rep_general in *.
+            logic_clean.
+            (** XXXX
+            erewrite map_addr_list_eq_map_map; eauto.
+            rewrite shift_list_upd_batch_set_comm; eauto.
+            erewrite <- shift_select_total_mem_synced.      
+            repeat rewrite <- shift_list_upd_batch_set_comm.        
+            repeat erewrite <- map_addr_list_eq_map_map; eauto.
+            
+            all: try apply sumbool_agree_addr_dec.
+            intros; apply H5; lia.
+             **)
+            admit.
+          }
+        }        
+        {
+          unfold cached_log_crash_rep in H1; cleanup.
+          edestruct recovery_simulation; eauto;
+          try solve [eapply H3; eauto].
+          {
+            unfold refines_to_reboot, cached_log_reboot_rep; simpl.          
+            split.          
+            eapply log_rep_to_reboot_rep in H1.
+            eexists; intuition eauto.
+            intros.
+            apply select_total_mem_synced in H3; eauto.
+          }
+          {
+            exists (Recovered (extract_state_r x)); simpl; intuition eauto.        
+            unfold logged_disk_reboot_list; simpl.
+            eapply ExecRecovered.
+            repeat econstructor.
+            unfold refines_to, cached_log_rep in *; simpl in *; cleanup; eauto.
+            rewrite <- H13; eauto.
+            erewrite <- shift_select_total_mem_synced; eauto.
+            intros; apply H4; lia.
+          }
+        }
+      }        
+      {(** After Commit case **)
+        specialize H4 with (1:= H0).
+        unfold cached_log_crash_rep in *; cleanup.
+        edestruct recovery_simulation; eauto;
+        try solve [eapply H3; eauto].
+        {
+          unfold refines_to_reboot, cached_log_reboot_rep; simpl.          
+          split.          
+          eapply log_rep_to_reboot_rep in H1.
+          eexists; intuition eauto.
+          intros.
+          apply select_total_mem_synced in H5; eauto.
+        }
+        {
+          exists (Recovered (extract_state_r x1)); simpl; intuition eauto.        
+          unfold logged_disk_reboot_list; simpl.
+          eapply ExecRecovered.
+          repeat econstructor; eauto.
+          (** Nodup goal for write crash **)
+          admit.
+          (** Length goal for write crash **)
+          admit.
+          (** Bound goal for write crash **)
+          admit.
+          (** Log length goal for write crash **)
+          admit.  
+          unfold refines_to, cached_log_rep in *; simpl in *; cleanup; eauto.
+          setoid_rewrite H3; eauto.
+          {
+            unfold log_rep, log_rep_general in H1.
+            
+            (** push shift inside then rewrite 
+                shift_select_total_mem_synced.
+             Too tired to do now. **)
+            admit.
+          }
+        }
+      }
+      {
+        specialize H3 with (1:= H0); cleanup.
+        split_ors; cleanup.
+        
+        {
+          unfold cached_log_reboot_rep in *; simpl in *;
+          cleanup.
+          edestruct recovery_simulation; eauto;
+          try solve [eapply H3; eauto].
+          {
+            unfold refines_to_reboot, cached_log_reboot_rep; simpl.
+            split.       
+            eexists; intuition eauto.
+            intros.
+            apply select_total_mem_synced in H4; eauto.
+          }
+          {
+            exists (Recovered (extract_state_r x1)); simpl; intuition eauto.        
+            unfold logged_disk_reboot_list; simpl.
+            eapply ExecRecovered.
+            repeat econstructor.
+            unfold refines_to, cached_log_rep in *; simpl in *; cleanup; eauto.
+          }
+        }        
+        {(** During Commit case **)
+          unfold cached_log_reboot_rep in *; simpl in *;
+          cleanup.
+          edestruct recovery_simulation; eauto;
+          try solve [eapply H3; eauto].
+          {
+            unfold refines_to_reboot, cached_log_reboot_rep; simpl.          
+            split.       
+            eexists; intuition eauto.
+            intros.
+            apply select_total_mem_synced in H6; eauto.
+          }
+          {
+            exists (Recovered (extract_state_r x1)); simpl; intuition eauto.        
+            unfold logged_disk_reboot_list; simpl.
+            eapply ExecRecovered.
+            repeat econstructor; eauto.
+            (** Nodup goal for write crash **)
+            admit.
+            (** Length goal for write crash **)
+            admit.
+            (** Bound goal for write crash **)
+            admit.
+            (** Log length goal for write crash **)
+            admit.  
+            unfold refines_to, cached_log_rep in *; simpl in *; cleanup; eauto.
+            setoid_rewrite H4; eauto.
+            }
+          }
+      }
+    }
+Admitted.
+
+
